Proved NoUninitialized_RunsTo

platform/cito/Wf.v
@@ -3,15 +3,424 @@
 
 Set Implicit Arguments.
 
+Require Import Bool.
+Require Import VariableLemmas SyntaxExpr SemanticsExpr Syntax Semantics.
+
+Fixpoint expReads (unwritten : string -> Prop) (e : Expr) (x : string) : Prop :=
+  match e with
+    | Var y => x = y /\ unwritten x
+    | Const _ => False
+    | Binop _ e1 e2 => expReads unwritten e1 x \/ expReads unwritten e2 x
+    | TestE _ e1 e2 => expReads unwritten e1 x \/ expReads unwritten e2 x
+  end.
+
+Import Syntax.
+
+Fixpoint writes (s : Stmt) (x : string) : Prop :=
+  match s with
+    | Assign y _ => x = y
+    | Label y _ => x = y
+    | Seq s1 s2 => writes s1 x \/ writes s2 x
+    | Skip => False
+    | Syntax.If _ s1 s2 => writes s1 x /\ writes s2 x
+    | Syntax.While _ _ => False
+    | Syntax.Call yo _ _ => match yo with
+                              | None => False
+                              | Some y => x = y
+                            end
+  end.
+
+Section ExistsR.
+  Variable A : Type.
+  Variable P : A -> Prop.
+
+  Fixpoint ExistsR (ls : list A) : Prop :=
+    match ls with
+      | nil => False
+      | x :: ls => P x \/ ExistsR ls
+    end.
+
+  Theorem ExistsR_Exists : forall ls, ExistsR ls -> List.Exists P ls.
+    induction ls; simpl; intuition.
+  Qed.
+
+  Theorem Exists_ExistsR : forall ls, List.Exists P ls -> ExistsR ls.
+    induction 1; simpl; intuition.
+  Qed.
+End ExistsR.
+
+Section ExistsR_weaken.
+  Variable A : Type.
+  Variables P Q : A -> Prop.
+
+  Hypothesis P_Q : forall x, P x -> Q x.
+
+  Theorem ExistsR_weaken : forall ls, ExistsR P ls -> ExistsR Q ls.
+    induction ls; simpl; intuition.
+  Qed.
+End ExistsR_weaken.
+
+Fixpoint reads (unwritten : string -> Prop) (s : Stmt) (x : string) : Prop :=
+  match s with
+    | Assign _ e => expReads unwritten e x
+    | Label _ _ => False
+    | Seq s1 s2 => reads unwritten s1 x \/ reads (fun x => unwritten x /\ ~writes s1 x) s2 x
+    | Skip => False
+    | Syntax.If e s1 s2 => expReads unwritten e x \/ reads unwritten s1 x \/ reads unwritten s2 x
+    | Syntax.While e s1 => expReads unwritten e x \/ reads unwritten s1 x
+    | Syntax.Call _ e1 es => expReads unwritten e1 x \/ ExistsR (fun e => expReads unwritten e x) es
+  end.
+
+Lemma eval_irrel : forall unwritten vs vs' e,
+  (forall x, ~expReads unwritten e x)
+  -> (forall x, sel vs' x <> sel vs x -> unwritten x)
+  -> eval vs e = eval vs' e.
+  induction e; simpl; intuition.
+  change (sel vs s = sel vs' s).
+  specialize (H0 s).
+  destruct (weq (sel vs' s) (sel vs s)).
+  eauto.
+  exfalso; eapply H.
+  descend.
+  eauto.
+  eauto.
+  f_equal; eauto.
+  rewrite IHe1 by eauto.
+  rewrite IHe2 by eauto.
+  auto.
+Qed.
+
+Local Hint Constructors RunsTo.
+
+Ltac irr E vs vs' :=
+  replace (eval vs E) with (eval vs' E) in *
+    by (eapply eval_irrel; (cbv beta; eauto)).
+
+Ltac irrel := simpl in *;
+  match goal with
+    | [ _ : context[eval ?vs' ?E] |- context[eval ?vs ?E ] ] =>
+      match vs with
+        | vs' => fail 1
+        | _ => irr E vs vs'
+      end
+  end.
+
+Lemma expReads_weaken : forall x (unwritten1 unwritten2 : _ -> Prop),
+  (forall y, unwritten1 y -> unwritten2 y)
+  -> forall e, expReads unwritten1 e x
+    -> expReads unwritten2 e x.
+  induction e; simpl; intuition.
+Qed.
+
+Ltac user' :=
+  try (eapply ExistsR_weaken; [ | eauto ]; cbv beta; intros);
+    match goal with
+      | _ => eapply expReads_weaken
+      | [ H : _ |- _ ] => eapply H
+    end; [ | solve [ eauto ] ]; cbv beta; solve [ intuition ].
+
+Ltac user := user' || (left; user) || (right; user).
+
+Lemma reads_weaken : forall x s (unwritten1 unwritten2 : _ -> Prop),
+  (forall y, unwritten1 y -> unwritten2 y)
+  -> reads unwritten1 s x
+  -> reads unwritten2 s x.
+  induction s; simpl; intuition eauto; user.
+Qed.
+
+Ltac use E := eapply E; [ | eauto ]; cbv beta; tauto.
+
+Section ADTValue.
+  Variable ADTValue : Type.
+
+  Lemma expReads_trivial : forall x e unwritten,
+    (forall x, ~unwritten x)
+    -> expReads unwritten e x
+    -> False.
+    induction e; simpl; intuition eauto.
+  Qed.
+
+  Hint Resolve expReads_trivial.
+
+  Lemma reads_trivial' : forall x s unwritten,
+    (forall x, ~unwritten x)
+    -> ~reads unwritten s x.
+    induction s; simpl; intuition; eauto.
+    eapply IHs2.
+    2: eauto.
+    simpl; intuition eauto.
+    induction l; simpl in *; intuition eauto.
+  Qed.
+
+  Lemma reads_trivial : forall x s,
+    ~reads (fun _ => False) s x.
+    intros; apply reads_trivial'; auto.
+  Qed.
+
+  Lemma prove_NoUninitializedRunsTo' : forall fs s st st', RunsTo (ADTValue := ADTValue) fs s st st'
+  -> forall unwritten vs'', (forall x, ~reads unwritten s x)
+    -> (forall x, sel vs'' x <> sel (fst st) x -> unwritten x)
+    -> exists vs''', RunsTo fs s (vs'', snd st) (vs''', snd st')
+      /\ (forall x, sel vs''' x <> sel (fst st') x -> unwritten x /\ ~writes s x).
+    induction 1; simpl; intuition;
+      repeat match goal with
+               | [ x := _ |- _ ] => subst x
+             end; eauto.
+
+    edestruct (IHRunsTo1 unwritten); clear IHRunsTo1; eauto; intuition idtac.
+    edestruct (IHRunsTo2 (fun x => unwritten x /\ ~writes a x)); eauto; intuition idtac.
+    eexists; split.
+    eauto.
+    firstorder.
+
+    edestruct IHRunsTo; eauto; intuition idtac.
+    eexists; split.
+    econstructor; repeat irrel; eauto.
+    firstorder.
+
+    edestruct IHRunsTo; eauto; intuition idtac.
+    eexists; split.
+    eapply RunsToIfFalse; repeat irrel; eauto.
+    firstorder.
+
+    edestruct IHRunsTo.
+    Focus 3.
+    intuition.
+    eexists; split.
+    eauto.
+    intros.
+    apply H4 in H2.
+    destruct H2; split.
+    apply H2.
+    auto.
+    simpl; intuition eauto.
+    eapply H0.
+    left.
+    use expReads_weaken.
+    eapply H0.
+    right.
+    use reads_weaken.
+    auto.
+
+    edestruct IHRunsTo.
+    Focus 3.
+    intuition idtac.
+    eexists; split.
+    econstructor.
+    simpl; irrel; eauto.
+    simpl.
+
+    Lemma map_eval_irrel : forall unwritten vs vs' es,
+      (forall x, ~ExistsR (fun e => expReads unwritten e x) es)
+      -> (forall x, sel vs' x <> sel vs x -> unwritten x)
+      -> map (eval vs) es = map (eval vs') es.
+      induction es; simpl; intuition.
+      f_equal.
+      eapply eval_irrel; eauto.
+      eauto.
+    Qed.
+
+    erewrite <- map_eval_irrel; eauto.
+    eauto.
+    simpl.
+    intros.
+    destruct var; simpl in *.
+    2: eauto.
+    destruct (string_dec s x0); subst.
+    Focus 2.
+    repeat rewrite sel_upd_ne in H4 by auto.
+    eauto.
+    repeat rewrite sel_upd_eq in H4 by reflexivity.
+    apply H6 in H4.
+    generalize dependent H4.
+    instantiate (1 := fun _ => False); simpl in *.
+    intuition.
+    2: tauto.
+    intro; apply reads_trivial.
+
+    eexists; split.
+    change (heap_upd_option
+      (fold_left (store_out (ADTValue:=ADTValue)) triples (snd v))
+      (fst (decide_ret addr ret)) (snd (decide_ret addr ret)))
+    with (heap_upd_option (fold_left (@store_out _) triples (snd (vs'', snd v)))
+      (fst (decide_ret addr ret)) (snd (decide_ret addr ret))).
+    eapply RunsToCallForeign; simpl.
+    simpl; irrel; eauto.
+    simpl; erewrite <- map_eval_irrel; eauto.
+    eauto.
+    simpl.
+    auto.
+    auto.
+    auto.
+    intros.
+    destruct var; simpl in *.
+    2: eauto.
+    destruct (string_dec s x); subst.
+    Focus 2.
+    repeat rewrite sel_upd_ne in H7 by auto.
+    eauto.
+    repeat rewrite sel_upd_eq in H7 by reflexivity.
+    tauto.
+
+    eexists; split.
+    change (snd v) with (snd (vs'', snd v)) at 2.
+    eauto.
+    simpl; intros.
+    destruct (string_dec x0 x); subst.
+    repeat rewrite sel_upd_eq in H0 by reflexivity; tauto.
+    repeat rewrite sel_upd_ne in H0 by auto.
+    eauto.
+
+    eexists; split.
+    change (snd v) with (snd (vs'', snd v)) at 2.
+    econstructor.
+    simpl; intros.
+    destruct (string_dec x0 x); subst.
+    repeat rewrite sel_upd_eq in H1 by reflexivity.
+    exfalso; apply H1.
+    irrel; auto.
+    repeat rewrite sel_upd_ne in H1 by auto.
+    eauto.
+  Qed.
+
+  Theorem prove_NoUninitializedRunsTo : forall arg_vars s,
+    (forall x, ~reads (fun s => ~In s arg_vars) s x)
+    -> forall fs vs a vs' a', RunsTo (ADTValue := ADTValue) fs s (vs, a) (vs', a')
+      -> forall vs'', agree_on vs vs'' arg_vars
+        -> exists vs''', RunsTo fs s (vs'', a) (vs''', a').
+    intros.
+    eapply prove_NoUninitializedRunsTo' in H0; eauto.
+    Focus 2.
+    instantiate (1 := vs''); simpl in *.
+    unfold not; intros.
+    eapply Forall_forall in H1; eauto.
+    firstorder.
+  Qed.
+
+  (*Local Hint Constructors Safety.Safe.
+
+  Lemma prove_NoUninitializedSafe' : forall s unwritten,
+    (forall x, ~reads unwritten s x)
+    -> forall fs vs a, Safety.Safe fs s (vs, a)
+      -> forall vs', (forall x, sel vs' x <> sel vs x -> unwritten x)
+        -> Safety.Safe fs s (vs', a).
+    intros; apply (@Safety.Safe_coind fs (fun s st =>
+      exists unwritten,
+        (forall x, ~reads unwritten s x)
+        /\ exists vs, Safety.Safe fs s (vs, snd st)
+          /\ (forall x, sel (fst st) x <> sel vs x -> unwritten x)));
+    intuition idtac;
+      repeat match goal with
+               | [ H : Logic.ex _ |- _ ] => destruct H; intuition idtac
+             end; simpl in *;
+      match goal with
+        | [ H : Safety.Safe _ _ _ |- _ ] => inversion H; clear H;
+          repeat match goal with
+                   | [ x : _ |- _ ] => subst x
+                 end; simpl in *; cbv beta; intuition idtac
+      end.
+
+    repeat irrel; auto.
+    repeat irrel; auto.
+    eauto 10.
+
+    eapply prove_NoUninitializedRunsTo' in H3; eauto.
+    destruct H3; intuition idtac.
+    repeat esplit; eauto.
+    intros.
+    apply (H5 _ (not_eq_sym H2)).
+    eauto.
+
+    left; repeat irrel; eauto 10.
+
+    right; repeat irrel; eauto 10.
+
+    left; repeat irrel; intuition idtac.
+    eauto 10.
+    eapply prove_NoUninitializedRunsTo' in H2; eauto.
+    destruct H2; intuition idtac.
+    repeat esplit; eauto.
+    firstorder.
+    firstorder.
+
+    repeat irrel; eauto.
+
+    repeat irrel; auto.
+
+    repeat irrel; auto.
+
+    repeat irrel; auto.
+
+    repeat irrel; eauto.
+
+    right; repeat irrel.
+    repeat esplit.
+    eauto.
+    3: instantiate (2 := vs_arg).
+    3: tauto.
+    2: eauto.
+
+    Lemma expReads_trivial : forall x e unwritten,
+      (forall x, ~unwritten x)
+      -> expReads unwritten e x
+      -> False.
+      induction e; simpl; intuition eauto.
+    Qed.
+
+    Hint Resolve expReads_trivial.
+
+    Lemma reads_trivial' : forall x s unwritten,
+      (forall x, ~unwritten x)
+      -> ~reads unwritten s x.
+      induction s; simpl; intuition; eauto.
+      eapply IHs2.
+      2: eauto.
+      simpl; intuition eauto.
+    Qed.
+
+    Lemma reads_trivial : forall x s,
+      ~reads (fun _ => False) s x.
+      intros; apply reads_trivial'; auto.
+    Qed.
+
+    intros.
+    apply reads_trivial in H4; tauto.
+
+    eauto 6.
+    eauto 6.
+    eauto 6.
+    eauto 6.
+    eauto 6.
+    eauto 6.
+    eauto 6.
+    eauto 6.
+    eauto 6.
+    eauto 6.
+    eauto 6.
+    eauto 6.
+    eauto 6.
+    eauto 6.
+  Qed.    
+
+  Theorem prove_NoUninitializedSafe : forall s,
+    (forall x, ~reads (fun s => s <> "__arg")%type s x)
+    -> forall fs vs a, Safety.Safe fs s (vs, a)
+      -> forall vs', sel vs' "__arg" = sel vs "__arg"
+        -> Safety.Safe fs s (vs', a).
+    intros.
+    eapply prove_NoUninitializedSafe' in H0; eauto.
+    firstorder.
+  Qed.*)
+End ADTValue.
+
 Section TopSection.
 
   Require Import Syntax.
   Require Import Locals.
   Require Import String.
 
-  Definition NoUninitialized : list string -> Stmt -> Prop.
-    admit.
-  Qed.
+  Definition NoUninitialized (arg_vars : list string) (s : Stmt) :=
+    forall x, ~reads (fun s => ~In s arg_vars) s x.
 
   Definition agree_in vs vs' vars := List.Forall (fun x => sel vs x = sel vs' x) vars.
 
@@ -38,298 +447,13 @@ Module Make (Import E : ADT).
       admit.
     Qed.
 
-    Lemma NoUninitialized_RunsTo : forall arg_vars s, NoUninitialized arg_vars s -> forall fs vs h v', RunsTo fs s (vs, h) v' -> forall vs', agree_in vs vs' arg_vars -> RunsTo fs s (vs', h) v'.
-      admit.
+    Lemma NoUninitialized_RunsTo : forall arg_vars s, NoUninitialized arg_vars s -> forall fs vs h v', RunsTo fs s (vs, h) v' -> forall vs', agree_in vs vs' arg_vars ->
+      exists vs'', RunsTo fs s (vs', h) (vs'', snd v').
+      intros.
+      destruct v'; simpl.
+      eapply prove_NoUninitializedRunsTo in H0; eauto.
     Qed.
     
   End TopSection.
 
 End Make.
-
-(*
-Require Import Bool.
-Require Import VariableLemmas SyntaxExpr SemanticsExpr Syntax Semantics.
-
-Fixpoint expReads (unwritten : string -> Prop) (e : Expr) (x : string) : Prop :=
-  match e with
-    | Var y => x = y /\ unwritten x
-    | Const _ => False
-    | Binop _ e1 e2 => expReads unwritten e1 x \/ expReads unwritten e2 x
-    | TestE _ e1 e2 => expReads unwritten e1 x \/ expReads unwritten e2 x
-  end.
-
-Import Syntax.
-
-Fixpoint writes (s : Statement) (x : string) : Prop :=
-  match s with
-    | Assignment y _ => x = y
-    | ReadAt y _ _ => x = y
-    | WriteAt _ _ _ => False
-    | Seq s1 s2 => writes s1 x \/ writes s2 x
-    | Skip => False
-    | Conditional _ s1 s2 => writes s1 x /\ writes s2 x
-    | Loop _ _ => False
-    | Malloc y _ => x = y
-    | Free _ => False
-    | Len y _ => x = y
-    | Syntax.Call _ _ => False
-  end.
-
-Fixpoint reads (unwritten : string -> Prop) (s : Statement) (x : string) : Prop :=
-  match s with
-    | Assignment _ e => expReads unwritten e x
-    | ReadAt _ e1 e2 => expReads unwritten e1 x \/ expReads unwritten e2 x
-    | WriteAt e1 e2 e3 => expReads unwritten e1 x \/ expReads unwritten e2 x \/ expReads unwritten e3 x
-    | Seq s1 s2 => reads unwritten s1 x \/ reads (fun x => unwritten x /\ ~writes s1 x) s2 x
-    | Skip => False
-    | Conditional e s1 s2 => expReads unwritten e x \/ reads unwritten s1 x \/ reads unwritten s2 x
-    | Loop e s1 => expReads unwritten e x \/ reads unwritten s1 x
-    | Malloc _ e => expReads unwritten e x
-    | Free e => expReads unwritten e x
-    | Len _ e => expReads unwritten e x
-    | Syntax.Call e1 e2 => expReads unwritten e1 x \/ expReads unwritten e2 x
-  end.
-
-Lemma exprDenote_irrel : forall unwritten vs vs' e,
-  (forall x, ~expReads unwritten e x)
-  -> (forall x, sel vs' x <> sel vs x -> unwritten x)
-  -> exprDenote e vs = exprDenote e vs'.
-  induction e; simpl; intuition.
-  change (sel vs s = sel vs' s).
-  specialize (H0 s).
-  destruct (weq (sel vs' s) (sel vs s)); eauto.
-  exfalso; eauto.
-  f_equal; eauto.
-  rewrite IHe1 by eauto.
-  rewrite IHe2 by eauto.
-  auto.
-Qed.
-
-Local Hint Constructors RunsTo.
-
-Ltac irr E vs vs' :=
-  replace (exprDenote E vs) with (exprDenote E vs') in *
-    by (eapply exprDenote_irrel; (cbv beta; eauto)).
-
-Ltac irrel := simpl in *;
-  match goal with
-    | [ _ : context[exprDenote ?E ?vs'] |- context[exprDenote ?E ?vs] ] =>
-      match vs with
-        | vs' => fail 1
-        | _ => irr E vs vs'
-      end
-  end.
-
-Lemma prove_NoUninitializedRunsTo' : forall fs s st st', RunsTo fs s st st'
-  -> forall unwritten vs'', (forall x, ~reads unwritten s x)
-    -> (forall x, sel vs'' x <> sel (fst st) x -> unwritten x)
-    -> exists vs''', RunsTo fs s (vs'', snd st) (vs''', snd st')
-      /\ (forall x, sel vs''' x <> sel (fst st') x -> unwritten x /\ ~writes s x).
-  induction 1; simpl; intuition;
-    repeat match goal with
-             | [ x := _ |- _ ] => subst x
-           end; eauto.
-
-  eexists; split.
-  econstructor; repeat irrel; auto.
-  intros.
-  destruct (string_dec var x); subst; autorewrite with sepFormula in *; eauto.
-  exfalso; apply H2.
-  eapply exprDenote_irrel; (cbv beta; eauto).
-
-  eexists; split.
-  econstructor.
-  repeat irrel; auto.
-  intros.
-  destruct (string_dec var x); subst; autorewrite with sepFormula in *; eauto.
-  exfalso; apply H3.
-  f_equal.
-  irrel; auto.
-  irrel; auto.
-
-  eexists; split.
-  irr arr vs vs''.
-  irr idx vs vs''.
-  irr value vs vs''.
-  econstructor.
-  repeat irrel; auto.
-  auto.
-
-  edestruct (IHRunsTo1 unwritten); clear IHRunsTo1; eauto; intuition idtac.
-  edestruct (IHRunsTo2 (fun x => unwritten x /\ ~writes a x)); eauto; intuition idtac.
-  eexists; split.
-  eauto.
-  firstorder.
-
-  edestruct IHRunsTo; eauto; intuition idtac.
-  eexists; split.
-  econstructor; repeat irrel; eauto.
-  firstorder.
-
-  edestruct IHRunsTo; eauto; intuition idtac.
-  eexists; split.
-  econstructor 7; repeat irrel; eauto.
-  firstorder.
-
-  edestruct (IHRunsTo1 unwritten); clear IHRunsTo1; eauto; intuition idtac.
-  edestruct (IHRunsTo2 unwritten x); eauto; intuition idtac.
-  specialize (H6 _ H4); tauto.
-  eexists; split.
-  econstructor; repeat irrel; eauto.
-  firstorder.
-
-  eexists; split.
-  econstructor 9; repeat irrel; eauto.
-  firstorder.
-
-  eexists; split.
-  econstructor; repeat irrel; eauto.
-  intros.
-  destruct (string_dec var x); subst; autorewrite with sepFormula in *; eauto.
-
-  eexists; split.
-  irr arr vs vs''.
-  econstructor; repeat irrel; eauto.
-  firstorder.
-
-  eexists; split.
-  econstructor; repeat irrel; eauto.
-  intros.
-  destruct (string_dec var x); subst; autorewrite with sepFormula in *; eauto.
-  irr arr vs'' vs; tauto.
-
-  eexists; split.
-  econstructor; repeat irrel; eauto.
-  firstorder.
-
-  eexists; split.
-  econstructor 14; repeat irrel; eauto.
-  firstorder.
-Qed.  
-
-Theorem prove_NoUninitializedRunsTo : forall s,
-  (forall x, ~reads (fun s => s <> "__arg")%type s x)
-  -> forall fs vs a vs' a', RunsTo fs s (vs, a) (vs', a')
-    -> forall vs'', sel vs'' "__arg" = sel vs "__arg"
-      -> exists vs''', RunsTo fs s (vs'', a) (vs''', a').
-  intros.
-  eapply prove_NoUninitializedRunsTo' in H0; eauto.
-  2: instantiate (1 := vs''); simpl in *; congruence.
-  firstorder.
-Qed.
-
-Local Hint Constructors Safety.Safe.
-
-Lemma prove_NoUninitializedSafe' : forall s unwritten,
-  (forall x, ~reads unwritten s x)
-  -> forall fs vs a, Safety.Safe fs s (vs, a)
-    -> forall vs', (forall x, sel vs' x <> sel vs x -> unwritten x)
-      -> Safety.Safe fs s (vs', a).
-  intros; apply (@Safety.Safe_coind fs (fun s st =>
-    exists unwritten,
-      (forall x, ~reads unwritten s x)
-      /\ exists vs, Safety.Safe fs s (vs, snd st)
-        /\ (forall x, sel (fst st) x <> sel vs x -> unwritten x)));
-  intuition idtac;
-    repeat match goal with
-             | [ H : Logic.ex _ |- _ ] => destruct H; intuition idtac
-           end; simpl in *;
-    match goal with
-      | [ H : Safety.Safe _ _ _ |- _ ] => inversion H; clear H;
-        repeat match goal with
-                 | [ x : _ |- _ ] => subst x
-               end; simpl in *; cbv beta; intuition idtac
-    end.
-
-  repeat irrel; auto.
-  repeat irrel; auto.
-  eauto 10.
-
-  eapply prove_NoUninitializedRunsTo' in H3; eauto.
-  destruct H3; intuition idtac.
-  repeat esplit; eauto.
-  intros.
-  apply (H5 _ (not_eq_sym H2)).
-  eauto.
-
-  left; repeat irrel; eauto 10.
-
-  right; repeat irrel; eauto 10.
-
-  left; repeat irrel; intuition idtac.
-  eauto 10.
-  eapply prove_NoUninitializedRunsTo' in H2; eauto.
-  destruct H2; intuition idtac.
-  repeat esplit; eauto.
-  firstorder.
-  firstorder.
-
-  repeat irrel; eauto.
-
-  repeat irrel; auto.
-
-  repeat irrel; auto.
-
-  repeat irrel; auto.
-
-  repeat irrel; eauto.
-
-  right; repeat irrel.
-  repeat esplit.
-  eauto.
-  3: instantiate (2 := vs_arg).
-  3: tauto.
-  2: eauto.
-
-  Lemma expReads_trivial : forall x e unwritten,
-    (forall x, ~unwritten x)
-    -> expReads unwritten e x
-    -> False.
-    induction e; simpl; intuition eauto.
-  Qed.
-
-  Hint Resolve expReads_trivial.
-
-  Lemma reads_trivial' : forall x s unwritten,
-    (forall x, ~unwritten x)
-    -> ~reads unwritten s x.
-    induction s; simpl; intuition; eauto.
-    eapply IHs2.
-    2: eauto.
-    simpl; intuition eauto.
-  Qed.
-
-  Lemma reads_trivial : forall x s,
-    ~reads (fun _ => False) s x.
-    intros; apply reads_trivial'; auto.
-  Qed.
-
-  intros.
-  apply reads_trivial in H4; tauto.
-
-  eauto 6.
-  eauto 6.
-  eauto 6.
-  eauto 6.
-  eauto 6.
-  eauto 6.
-  eauto 6.
-  eauto 6.
-  eauto 6.
-  eauto 6.
-  eauto 6.
-  eauto 6.
-  eauto 6.
-  eauto 6.
-Qed.    
-
-Theorem prove_NoUninitializedSafe : forall s,
-  (forall x, ~reads (fun s => s <> "__arg")%type s x)
-  -> forall fs vs a, Safety.Safe fs s (vs, a)
-    -> forall vs', sel vs' "__arg" = sel vs "__arg"
-      -> Safety.Safe fs s (vs', a).
-  intros.
-  eapply prove_NoUninitializedSafe' in H0; eauto.
-  firstorder.
-Qed.
- *)
